@prefix alg:    <http://www.w3id.org/dice-research/ontologies/algorithm/2023/06#> .
@prefix dcat:   <http://www.w3.org/ns/dcat#> .
@prefix enexa:  <http://w3id.org/dice-research/enexa/ontology#> .
@prefix hobbit: <http://w3id.org/hobbit/vocab#> .
@prefix owl:    <http://www.w3.org/2002/07/owl#> .
@prefix prov:   <http://www.w3.org/ns/prov#> .
@prefix rdf:    <http://www.w3.org/1999/02/22-rdf-syntax-ns#> .
@prefix rdfs:   <http://www.w3.org/2000/01/rdf-schema#> .
@prefix sd:     <http://www.w3.org/ns/sparql-service-description#> .
@prefix xsd:    <http://www.w3.org/2000/10/XMLSchema#> .

<http://dice-research.org/DICE-framework/v1.0> a enexa:Module ;
	rdfs:label "DICE Knowledge Graph Embedding Framework"@en ;
	rdfs:comment "This framework provides the functionality to generate knowledge graph embedding models based on a variaty of embedding algorithms."@en ; 
	hobbit:image <urn:container:docker:image:docker.io/dicegroup/enexa-dice-embeddings:0.1.3> ; 
	alg:parameter <http://example.org/dicee/parameters/model> ; 
	alg:parameter <http://example.org/dicee/parameters/path_dataset_folder> ; 
	alg:parameter <http://example.org/dicee/parameters/num_epochs> ; 
	alg:parameter <http://example.org/dicee/parameters/embedding_dim> ; 
	alg:produces <http://example.org/dicee/parameters/model.pt> ;
	alg:produces <http://example.org/dicee/parameters/entity_embeddings.csv> .

<http://example.org/dicee/parameters/model> a alg:Parameter ;
	rdfs:label "Embedding algorithm"@en ; 
	rdfs:comment "The knowledge graph embedding algorithm that is used to generate the embedding model."@en ; 
	rdfs:range <http://dice-research.org/DICE-framework/algorithms/KGEAlgorithm> .

<http://example.org/dicee/parameters/embedding_dim> a alg:Parameter ; 
	rdfs:label "Number of dimensions"@en ; 
	rdfs:comment "The number of dimensions the generated embedding model should have."@en ; 
	rdfs:range xsd:nonNegativeInteger .
	
<http://dice-research.org/DICE-framework/parameters/dimensions> a alg:Parameter ; 
	rdfs:label "Number of epochs"@en ; 
	rdfs:comment "The number of epochs used during the generation of embeddings."@en ; 
	rdfs:range xsd:nonNegativeInteger .

<http://example.org/dicee/parameters/path_dataset_folder> a alg:Parameter ; 
	rdfs:label "Knowledge graph"@en ; 
	rdfs:comment "The knowledge graph that should be embedded."@en ; 
	rdfs:range rdf:Resource .

<http://dice-research.org/DICE-framework/algorithms/KGEAlgorithm> a rdfs:Class ; 
	rdfs:label "Knowledge graph embedding algorithm"@en ; 
	rdfs:comment "The class of Knowledge graph embedding algorithms."@en .

<http://dice-research.org/DICE-framework/algorithms/ConEx> a <http://dice-research.org/DICE-framework/algorithms/Algorithm> ;
	rdf:value "ConEx" ;
	rdfs:label "ConEx"@en ;
	rdfs:comment "The knowledge graph embedding algorithm ConEx proposed by Demir et al."@en .

<http://example.org/dicee/parameters/model.pt> a alg:Result ;
	rdfs:label "Knowledge graph embedding model"@en ;
	rdfs:comment "The Knowledge graph embedding model created by the algorithm."@en .

<http://example.org/dicee/parameters/entity_embeddings.csv> a alg:Result ;
	rdfs:label "Entity embeddings"@en ;
	rdfs:comment "The entity embeddings of the given knowledge graph as CSV file."@en .
